replace.sh
@@ -4,7 +4,7 @@ echo $1
 echo $2
 
 ${SED} -i -E -e \
-    "s/declared_inductive (((\.*\))|([^ _]*)) ([^ ]*) ([^ ]*) ([^ ]*)([\(| ->])/declared_inductive \1 \5 \3 \6\7/g" \
+    "s/declared_inductive ((\(.*\))|[^ ]*) ((\(.*\))|[^ ]*) ((\(.*\))|[^ ]*) ((\(.*\))|[^ ]*)([\)| ->])/declared_inductive \1 \5 \3 \7\9/g" \
     */*/*.v
 
 # ${SED} -i -e "s/${1}/${2}/g" */*/*.v
